finish compile_fake_exp_val
excepting a cheat for the lemma about swapping in an equivalent source
language environment. not sure how easy that will be to prove, but
hoping it's true. also hoping this statement of compile_fake_exp_val is
good enough for compile_dec.

compiler/proofs/compilerProofsScript.sml
@@ -377,20 +377,31 @@ val EVERY2_DROP = store_thm("EVERY2_DROP",
   match_mp_tac (MP_CANON EVERY_DROP) >>
   rw[] >> PROVE_TAC[])
 
+val vlabs_list_APPEND = store_thm("vlabs_list_APPEND",
+  ``vlabs_list (l1 ++ l2) = vlabs_list l1 ∪ vlabs_list l2``,
+  rw[vlabs_list_MAP])
+
+val vlabs_list_REVERSE = store_thm("vlabs_list_REVERSE",
+  ``vlabs_list (REVERSE ls) = vlabs_list ls``,
+  rw[vlabs_list_MAP])
+
+val closed_under_menv_def = Define`
+  closed_under_menv menv env s ⇔
+    EVERY (closed menv) s ∧
+    EVERY (closed menv) (MAP SND env) ∧
+    EVERY (EVERY (closed menv) o MAP SND) (MAP SND menv)`
+
 val compile_fake_exp_val = store_thm("compile_fake_exp_val",
-  ``∀menv cenv s env expf exp s' vs rd rs vars vv0 vv1 rs' bc0 bc bs bs'.
+  ``∀rs vars expf menv cenv s env exp s' vs rs' bc rd vv0 vv1 bc0 bs.
       evaluate menv cenv s env exp (s', Rval (Conv (Short "") vs)) ∧
       is_null menv ∧
-      EVERY (closed menv) s ∧
-      EVERY (closed menv) (MAP SND env) ∧
-      EVERY (EVERY (closed menv) o MAP SND) (MAP SND menv) ∧
       FV exp ⊆ set (MAP (Short o FST) env) ∪ menv_dom menv ∧
+      closed_under_menv menv env s ∧
       closed_under_cenv cenv menv env s ∧
       (∀v. v ∈ env_range env ∨ MEM v s ⇒ all_locs v ⊆ count (LENGTH s)) ∧
       LENGTH s' ≤ LENGTH rd.sm ∧
       env_rs cenv env rs rd s (bs with code := bc0) ∧
-      ALL_DISTINCT vars ∧
-      (LENGTH vars = LENGTH vs) ∧
+      ALL_DISTINCT vars ∧ (LENGTH vars = LENGTH vs) ∧
       (PARTITION (λv. MEM v rs.rbvars) vars = (vv0,vv1)) ∧
       (compile_fake_exp rs vars expf = (rs',bc)) ∧
       (exp = expf (Con (Short "") (MAP (Var o Short) (vv0++vv1)))) ∧
@@ -430,6 +441,7 @@ val compile_fake_exp_val = store_thm("compile_fake_exp_val",
   qspecl_then[`menv`,`cenv`,`s`,`env1`,`exp`,`(s1,Rval (Conv (Short "") vs1))`] mp_tac (CONJUNCT1 exp_to_Cexp_thm1) >>
   simp[] >>
   discharge_hyps >- (
+    fs[closed_under_menv_def] >>
     simp[Abbr`env1`] >>
     fsrw_tac[DNF_ss][SUBSET_DEF,MEM_MAP] >>
     fsrw_tac[DNF_ss][EVERY_MEM,MEM_MAP,closed_under_cenv_def,FORALL_PROD] >>
@@ -550,6 +562,13 @@ val compile_fake_exp_val = store_thm("compile_fake_exp_val",
   simp[Once Cv_bv_cases] >>
   disch_then(Q.X_CHOOSE_THEN`bvs`strip_assume_tac) >>
   last_x_assum(qspecl_then[`bs2 with code := bc0++c0++REVERSE bc1++c1 `,`bc0++c0++REVERSE bc1`,`4`,`bvs`,`bs.stack`]mp_tac) >>
+  `LENGTH rs.rbvars ≤ LENGTH bs.stack` by (
+    qpat_assum`Cenv_bs rd Cs Cenv renv (LENGTH rs.rbvars)X `mp_tac >>
+    simp[Cenv_bs_def,EVERY2_EVERY,Abbr`renv`,EVERY_MEM,FORALL_PROD,MEM_ZIP,GSYM LEFT_FORALL_IMP_THM,CompilerLibTheory.el_check_def]>>
+    strip_tac >>
+    spose_not_then strip_assume_tac >>
+    first_x_assum(qspec_then`LENGTH bs.stack`mp_tac) >>
+    simp[] ) >>
   discharge_hyps >- (
     simp[Abbr`bs2`] >>
     qpat_assum`PARTITION X Y = Z`(assume_tac o SYM) >>
@@ -562,13 +581,6 @@ val compile_fake_exp_val = store_thm("compile_fake_exp_val",
       qpat_assum`syneq Cv0 X`mp_tac >>
       qpat_assum`syneq X Cv0`mp_tac >>
       simp[Once IntLangTheory.syneq_cases] ) >>
-    conj_tac >- (
-      qpat_assum`Cenv_bs rd Cs Cenv renv (LENGTH rs.rbvars)X `mp_tac >>
-      simp[Cenv_bs_def,EVERY2_EVERY,Abbr`renv`,EVERY_MEM,FORALL_PROD,MEM_ZIP,GSYM LEFT_FORALL_IMP_THM,CompilerLibTheory.el_check_def]>>
-      strip_tac >>
-      spose_not_then strip_assume_tac >>
-      first_x_assum(qspec_then`LENGTH bs.stack`mp_tac) >>
-      simp[] ) >>
     simp[SUBSET_DEF] >>
     metis_tac[ALL_DISTINCT_PERM,PARTITION_DEF,PERM_PARTITION,ALL_DISTINCT_APPEND] ) >>
   strip_tac >>
@@ -621,28 +633,27 @@ val compile_fake_exp_val = store_thm("compile_fake_exp_val",
     simp[Abbr`bs2'`,SUM_APPEND,FILTER_APPEND,ADD1,Abbr`bs2`] ) >>
   simp[Abbr`bs5`] >>
   ntac 5 (pop_assum kall_tac) >>
-  conj_tac >- (
-    qpat_assum`PARTITION X Y = Z`(assume_tac o SYM) >>
-    fs[PARTITION_DEF]>>
-    imp_res_tac PART_LENGTH >>
-    imp_res_tac PART_MEM >>
-    imp_res_tac PARTs_HAVE_PROP >>
-    fs[MAP_ZIP] >>
-    fs[EXTENSION] >> metis_tac[] ) >>
-  conj_tac >- (
-    simp[ALL_DISTINCT_APPEND,ALL_DISTINCT_REVERSE] >>
-    qpat_assum`PARTITION X Y = Z`(mp_tac o SYM) >>
-    qpat_assum`ALL_DISTINCT vars`mp_tac >>
-    qpat_assum`set rs.rbvars = X`(SUBST1_TAC o SYM) >>
-    rpt (pop_assum kall_tac) >>
-    simp[PARTITION_DEF] >>
-    rw[] >> imp_res_tac PART_MEM >>
-    imp_res_tac PARTs_HAVE_PROP >>
-    imp_res_tac PERM_PART >> fs[] >>
-    metis_tac[ALL_DISTINCT_PERM,ALL_DISTINCT_APPEND] ) >>
-  conj_tac >- metis_tac[EVERY2_syneq_trans] >>
   `LENGTH vs = LENGTH vv0 + LENGTH vv1` by
     metis_tac[PART_LENGTH,PARTITION_DEF,LENGTH_NIL,ADD_0,ADD_SYM] >>
+  `∀x. MEM x (vars ++ ([] ++ [])) ⇔ MEM x (vv0 ++ vv1)` by
+    metis_tac[PART_MEM,PARTITION_DEF] >>
+  `(∀x. MEM x vv0 ⇒ (λv. MEM v rs.rbvars) x) ∧
+   (∀x. MEM x vv1 ⇒ ¬ (λv. MEM v rs.rbvars) x)` by (
+    qpat_assum`PARTITION X Y = Z`(assume_tac o SYM) >>
+    qpat_assum`set rs.rbvars = X`kall_tac >>
+    fs[PARTITION_DEF] >>
+    imp_res_tac PARTs_HAVE_PROP >>
+    fs[] ) >>
+  `PERM vars (vv0 ++ vv1)` by metis_tac[PERM_PARTITION] >>
+  `ALL_DISTINCT (vv0 ++ vv1)` by (
+    metis_tac[ALL_DISTINCT_PERM] ) >>
+  fs[] >>
+  conj_tac >- ( fs[MAP_ZIP] >> fs[EXTENSION] >> metis_tac[] ) >>
+  conj_tac >- (
+    simp[ALL_DISTINCT_APPEND,ALL_DISTINCT_REVERSE] >>
+    qpat_assum`set rs.rbvars = X`(SUBST1_TAC o SYM) >>
+    metis_tac[ALL_DISTINCT_PERM,ALL_DISTINCT_APPEND] ) >>
+  conj_tac >- metis_tac[EVERY2_syneq_trans] >>
   conj_tac >- (
     match_mp_tac EVERY2_APPEND_suff >>
     conj_tac >- (
@@ -653,23 +664,18 @@ val compile_fake_exp_val = store_thm("compile_fake_exp_val",
       reverse conj_tac >- (
         match_mp_tac EVERY2_DROP >>
         simp[] >>
-        conj_tac >- metis_tac[EVERY2_syneq_trans] >>
-        qsuff_tac`LENGTH (vv0 ++ vv1) = LENGTH vars`>-simp[] >>
-        metis_tac[PERM_PARTITION,PERM_LENGTH] ) >>
+        metis_tac[EVERY2_syneq_trans]) >>
       simp[MAP_MAP_o,combinTheory.o_DEF] >>
       qmatch_abbrev_tac`LIST_REL R l1 l2` >>
       qsuff_tac`l1 = l2`>-metis_tac[EVERY2_syneq_refl] >>
       simp[Abbr`l1`,Abbr`l2`,LIST_EQ_REWRITE] >>
-      fs[EVERY2_EVERY,PARTITION_DEF] >>
-      `LENGTH vs = LENGTH vv0 + LENGTH vv1` by (
-        qpat_assum`X = (vv0,vv1)`(assume_tac o SYM) >>
-        imp_res_tac PART_LENGTH >> fs[] ) >>
-      simp[] >>
+      fs[EVERY2_EVERY] >>
       rw[EL_MAP] >>
       simp[EL_DROP,EL_MAP] >>
-      `ALL_DISTINCT (vv0 ++ vv1)` by (
-        metis_tac[ALL_DISTINCT_PERM,PERM_PART,APPEND_NIL] ) >>
-      ntac 3 (pop_assum mp_tac) >>
+      qunabbrev_tac`R` >>
+      ntac 2 (pop_assum mp_tac) >>
+      `LENGTH vs = LENGTH (vv0 ++ vv1)` by metis_tac[PERM_LENGTH] >>
+      pop_assum mp_tac >>
       rpt (pop_assum kall_tac) >>
       rw[] >>
       Q.PAT_ABBREV_TAC`al = ZIP (vv0++vv1,vs)` >>
@@ -769,8 +775,30 @@ val compile_fake_exp_val = store_thm("compile_fake_exp_val",
   conj_tac >- (
     fs[FORALL_PROD,EVERY_MEM] >>
     metis_tac[code_env_cd_append,APPEND_ASSOC] ) >>
-  conj_tac >- cheat >>
-  ntac 2 (pop_assum kall_tac) >>
+  conj_tac >- (
+    fs[GSYM FORALL_PROD] >>
+    qx_gen_tac`p` >> strip_tac >>
+    qsuff_tac `p ∈ vlabs_list Cvs ∨ p ∈ vlabs_list Cenv` >- (
+      fs[EVERY_MEM] >>
+      metis_tac[code_env_cd_append,APPEND_ASSOC] ) >>
+    fs[vlabs_list_APPEND,vlabs_list_REVERSE] >- (
+      disj1_tac >>
+      `LENGTH vv0 ≤ LENGTH Cvs` by (
+        fs[EVERY2_EVERY] >> simp[] ) >>
+      rfs[vlabs_list_MAP] >>
+      metis_tac[MEM_DROP] ) >>
+    fs[vlabs_list_MAP,MEM_GENLIST] >>
+    pop_assum mp_tac >> rw[] >- (
+      qmatch_assum_rename_tac`MEM z vv0`[] >>
+      Q.ISPECL_THEN[`vv0`,`z`,`0:num`]mp_tac find_index_MEM >>
+      rw[] >> fs[] >>
+      `i < LENGTH Cvs` by (
+        fs[EVERY2_EVERY] >> simp[] ) >>
+      metis_tac[MEM_EL] ) >>
+    qmatch_assum_rename_tac`p ∈ vlabs (EL i Cenv)`[] >>
+    `i < LENGTH Cenv` by ( fs[EVERY2_EVERY] >> simp[]) >>
+    metis_tac[MEM_EL] ) >>
+  ntac 3 (pop_assum kall_tac) >>
   Q.PAT_ABBREV_TAC`bsc:bc_state = X` >>
   match_mp_tac Cenv_bs_append_code >>
   qexists_tac`bsc with code := bc0 ++ c0` >>
@@ -783,7 +811,22 @@ val compile_fake_exp_val = store_thm("compile_fake_exp_val",
     fs[s_refs_def,good_rd_def,Abbr`bsc`] ) >>
   simp[Abbr`X`,Abbr`Y`,Abbr`Z`,Abbr`bsc`] >>
   fs[option_case_NONE_F] >>
-  cheat)
+  fs[EVERY2_EVERY] >>
+  conj_tac >- DECIDE_TAC >>
+  fs[EVERY_MEM,FORALL_PROD] >>
+  `LENGTH (DROP (LENGTH vv0) Cvs) = LENGTH vv1` by simp[] >>
+  rfs[MEM_ZIP,GSYM LEFT_FORALL_IMP_THM] >>
+  qx_gen_tac`n`>>strip_tac >>
+  simp[CompilerLibTheory.el_check_def] >>
+  Cases_on`n < LENGTH vv1`>>simp[EL_APPEND1,EL_APPEND2] >- (
+    simp[EL_REVERSE,PRE_SUB1,EL_DROP] ) >>
+  rw[] >- (
+    first_x_assum match_mp_tac >>
+    Q.ISPECL_THEN[`vv0`,`EL (n-LENGTH vv1) rs.rbvars`,`0:num`]mp_tac find_index_MEM >>
+    rw[] >> rw[] >> simp[] ) >>
+  qpat_assum`∀n. n < LENGTH rs.rbvars ⇒ X`(qspec_then`n - LENGTH vv1`mp_tac) >>
+  simp[Abbr`renv`,CompilerLibTheory.el_check_def] >>
+  simp[EL_CONS,PRE_SUB1])
 
 (* TODO: move?*)
 val FV_dec_def = Define`
